ambient_capabilities_coq_model/assert_theory.v
@@ -1,0 +1,31 @@
+Require Export Arith.
+Require Import List.
+Require Import Bool.
+
+Require Import CpdtTactics.
+Require Import common.
+Require Import language_def.
+Require Import assert.
+Require Export operational_semantics.
+
+Require Export Coq.Numbers.BinNums.
+Require Export ZArith.
+
+Module AssertTheory.
+
+  Import LanguageDefinition.
+  Import OperationalSemantics.
+  Import Assert.
+
+  Definition entails (M : module)(A1 A2 : asrt) : Prop := forall σ, sat M σ (A1 ⟶ A2).
+
+  Notation "M ⊢ A1 ⊆ A2" := (entails M A1 A2)(at level 40).
+
+  Lemma entails_strengthening :
+    forall M σ A1 A2, sat M σ A1 ->
+                 sat M σ (A1 ⟶ A2) ->
+                 sat M σ A2.
+  Proof.
+  Admitted.
+
+End AssertTheory.
